lamcalc

Lamcalc/Confluence.lean
@@ -1,8 +1,170 @@
 import Lamcalc.Semantics
+open ARS
+
+@[aesop safe [constructors, cases]]
+inductive pstep : tm -> tm -> Prop where
+| pstep_var x :
+  pstep (ids x) (ids x)
+| pstep_lam a {m m'} :
+  pstep m m' ->
+  pstep (.lam a m) (.lam a m')
+| pstep_app {m m' n n'} :
+  pstep m m' ->
+  pstep n n' ->
+  pstep (.app m n) (.app m' n')
+| pstep_beta a {m m' n n'} :
+  pstep m m' ->
+  pstep n n' ->
+  pstep (.app (.lam a m) n) (m'.[n'/])
+| pstep_unit :
+  pstep .unit .unit
+
+infix:50 " ≈> " => pstep
+
+def sred (σ τ : Nat -> tm) := ∀ x, (σ x) ~>* (τ x)
+
+lemma step_subst σ {m n} : m ~> n -> m.[σ] ~> n.[σ] := by
+  intro st
+  induction st generalizing σ <;> clear m n
+  case step_lam a m m' _ ih =>
+    simp; constructor
+    apply ih
+  case step_appM m m' n _ ih =>
+    simp; constructor
+    apply ih
+  case step_appN m n n' _ ih =>
+    simp; constructor
+    apply ih
+  case step_beta a m n =>
+    simp
+    rw [<-up_comp_subst]
+    rw [<-subst_comp]
+    apply step.step_beta
+
+lemma red_lam {a m m'} :
+  m ~>* m' -> .lam a m ~>* .lam a m' := by
+  intro r
+  apply star.hom (tm.lam a) _ r
+  intros x y
+  apply step.step_lam
+
+lemma red_app {m m' n n'} :
+  m ~>* m' -> n ~>* n' -> .app m n ~>* .app m' n' := by
+  intros r1 r2
+  apply (@star.trans _ _ (tm.app m' n))
+  . apply star.hom (tm.app · n) _ r1
+    intros x y; simp
+    apply step.step_appM
+  . apply star.hom _ _ r2
+    intros x y
+    apply step.step_appN
+
+lemma red_subst {m n} σ : m ~>* n -> m.[σ] ~>* n.[σ] := by
+  intro r
+  induction r with
+  | R => aesop
+  | SE _ st ih =>
+    apply star.trans ih
+    apply star.singleton
+    apply step_subst _ st
+
+lemma sred_up {σ τ} : sred σ τ -> sred (up σ) (up τ) := by
+  intros h x
+  cases x with
+  | zero => simp; aesop
+  | succ n =>
+    simp [up, funcomp, scons]
+    apply red_subst _ (h n)
+
+lemma red_compat {σ τ} m : sred σ τ -> m.[σ] ~>* m.[τ] := by
+  induction m generalizing σ τ with
+  | var x =>
+    simp; intro h
+    apply h
+  | lam a m ih =>
+    simp; intro h
+    apply red_lam (ih (sred_up h))
+  | app m n ihm ihn =>
+    simp; intro h
+    apply red_app (ihm h) (ihn h)
+  | unit => intro _; aesop
+
+def sconv (σ τ : Nat -> tm) := ∀ x, σ x === τ x
+
+lemma conv_lam {a m m'} :
+  m === m' -> tm.lam a m === tm.lam a m' := by
+  intros r; apply conv.hom _ _ r
+  intros x y; apply step.step_lam
+
+lemma conv_app {m m' n n'} :
+  m === m' -> n === n' -> tm.app m n === tm.app m' n' := by
+  intros r1 r2
+  apply @conv.trans _ _ (tm.app m' n)
+  . apply conv.hom (tm.app · n) _ r1
+    intros x y; simp
+    apply step.step_appM
+  . apply conv.hom _ _ r2
+    intros x y
+    apply step.step_appN
+
+lemma conv_subst σ {m n} : m === n -> m.[σ] === n.[σ] := by
+  intros r
+  apply conv.hom _ _ r
+  apply step_subst
+
+lemma sconv_up {σ τ} : sconv σ τ -> sconv (up σ) (up τ) := by
+  intros h x
+  cases x with
+  | zero => simp; aesop
+  | succ n =>
+    simp [up, funcomp, scons]
+    apply conv_subst _ (h n)
+
+lemma conv_compat {σ τ} m : sconv σ τ -> m.[σ] === m.[τ] := by
+  induction m generalizing σ τ with
+  | var x =>
+    simp; intro h; apply h
+  | lam a m ih =>
+    simp; intro h
+    apply conv_lam (ih (sconv_up h))
+  | app m n ihm ihn =>
+    simp; intro h
+    apply conv_app (ihm h) (ihn h)
+  | unit => simp; aesop
+
+lemma conv_beta {m n1 n2} : n1 === n2 -> m.[n1/] === m.[n2/] := by
+  intro h; apply conv_compat
+  intro x
+  cases x with
+  | zero => simp [scons]; assumption
+  | succ n => simp [scons]; aesop
 
 @[aesop safe]
 lemma pstep_refl {m} : m ≈> m := by
   induction m <;> aesop
+
+lemma step_pstep {m m'} : m ~> m' -> m ≈> m' := by
+  intro st
+  induction st with
+  | step_lam a _ ih => constructor; assumption
+  | step_appM _ ih => constructor <;> aesop
+  | step_appN _ ih => constructor <;> aesop
+  | step_beta a => constructor <;> aesop
+
+lemma pstep_red {m n} : m ≈> n -> m ~>* n := by
+  intro ps
+  induction ps <;> clear m n
+  case pstep_var x => aesop
+  case pstep_lam a m m' _ ih =>
+    apply red_lam ih
+  case pstep_app m m' n n' _ _ ihm ihn =>
+    apply red_app ihm ihn
+  case pstep_beta a m m' n n' _ _ ihm ihn =>
+    apply star.trans
+    . apply red_app (red_lam ihm) ihn
+    . apply star.singleton
+      apply step.step_beta
+  case pstep_unit => aesop
 
 lemma pstep_subst {m n} σ : m ≈> n -> m.[σ] ≈> n.[σ] := by
   intro ps
@@ -64,9 +226,8 @@ lemma pstep_compat_beta {m m' n n'} :
   . assumption
   . apply psstep_compat psstep_refl ps2
 
-lemma pstep_diamond {m m1 m2} :
-  m ≈> m1 -> m ≈> m2 -> ∃ m', m1 ≈> m' ∧ m2 ≈> m' := by
-  intro ps; induction ps generalizing m2 <;> clear m m1
+lemma pstep_diamond : diamond pstep := by
+  intros m m1 m2 ps; induction ps generalizing m2 <;> clear m m1
   case pstep_var x =>
     intro ps; exists m2; aesop
   case pstep_lam a m m' _ ih =>
@@ -118,3 +279,32 @@ lemma pstep_diamond {m m1 m2} :
     intro ps0; cases ps0
     exists tm.unit
     aesop
+
+lemma pstep_strip {m m1 m2} :
+  m ≈> m1 -> m ~>* m2 -> ∃ m', m1 ~>* m' ∧ m2 ≈> m' := by
+  intros p r
+  induction r generalizing m1 p <;> clear m2
+  case R =>
+    exists m1; constructor
+    . apply star.R
+    . assumption
+  case SE _ s1 ih =>
+    rcases ih p with ⟨m2, ⟨r, s2⟩⟩
+    rcases pstep_diamond (step_pstep s1) s2 with ⟨m3, ⟨p1, p2⟩⟩
+    exists m3; constructor
+    . apply star.trans r (pstep_red p2)
+    . assumption
+
+theorem step_confluent : confluent step := by
+  intros x y z r
+  induction r generalizing z <;> clear y
+  case R =>
+    intro h; exists z
+    constructor <;> aesop
+  case SE _ s ih =>
+    intro h
+    rcases ih h with ⟨z1, ⟨s1 , s2⟩⟩
+    rcases pstep_strip (step_pstep s) s1 with ⟨z2, ⟨s3, s4⟩⟩
+    exists z2; constructor
+    . assumption
+    . apply star.trans s2 (pstep_red s4)
