Lamcalc/ARS.lean
@@ -1,0 +1,187 @@
+import Mathlib.Tactic
+
+namespace ARS
+
+section ars_def
+set_option quotPrecheck false
+notation:70 e1:70 " <=2 " e2:70 => (∀ {x y}, e1 x y -> e2 x y)
+
+def Pred (T : Type) := T -> Prop
+def Rel (T : Type) := T -> Pred T
+attribute [reducible] Pred Rel
+
+variable {T : Type} (e : Rel T)
+
+inductive star (x : T) : T -> Prop where
+| R : star x x
+| SE {y z} : star x y -> e y z -> star x z
+
+inductive conv (x : T) : T -> Prop where
+| R : conv x x
+| SE  {y z} : conv x y -> e y z -> conv x z
+| SEi {y z} : conv x y -> e z y -> conv x z
+
+attribute [aesop unsafe] star.R conv.R
+
+def com (R S : Rel T) := ∀ {x y z}, R x y -> S x z -> ∃ u, S y u ∧ R z u
+def joinable (R : Rel T) x y := ∃ z, R x z ∧ R y z
+def diamond := ∀ {x y z}, e x y -> e x z -> ∃ u, e y u ∧ e z u
+def confluent := ∀ {x y z}, star e x y -> star e x z -> joinable (star e) y z
+def CR := ∀ {x y}, conv e x y -> joinable (star e) x y
+end ars_def
+
+section ars_lemmas
+variable {T : Type} {e : Rel T}
+
+lemma star.singleton {x y} : e x y -> star e x y := by
+  intro h
+  apply star.SE
+  apply star.R
+  assumption
+
+lemma star.trans {y x z} : star e x y -> star e y z -> star e x z := by
+  intros h1 h2
+  induction h2 with
+  | R => exact h1
+  | SE _ rel ih => apply star.SE ih rel
+
+lemma star.ES {x y z} : e x y -> star e y z -> star e x z := by
+  intro h
+  apply star.trans
+  apply star.singleton
+  assumption
+
+lemma star.conv {x y} : star e x y -> conv e x y := by
+  intro h
+  induction h with
+  | R => constructor
+  | SE _ rel ih => apply conv.SE ih rel
+
+lemma star.img {T1 T2} {f : T1 -> T2} {e1 e2} :
+  (∀ {x y}, e1 x y -> star e2 (f x) (f y)) ->
+  (∀ {x y}, star e1 x y -> star e2 (f x) (f y)) := by
+  intros h1 x y h2
+  induction h2 with
+  | R => aesop
+  | @SE y z _ rel ih => apply star.trans ih (h1 rel)
+
+lemma star.hom {T1 T2} (f : T1 -> T2) {e1 e2} :
+  (∀ {x y}, e1 x y -> e2 (f x) (f y)) ->
+  (∀ {x y}, star e1 x y -> star e2 (f x) (f y)) := by
+  intro h; apply star.img
+  intros x y h0
+  apply h at h0
+  apply star.singleton h0
+
+lemma star.closure {T} {e1 e2 : Rel T} : e1 <=2 star e2 -> star e1 <=2 star e2 := by
+  apply star.img
+
+lemma star.monotone {T} {e1 e2 : Rel T} : e1 <=2 e2 -> star e1 <=2 star e2 := by
+  intro h1; apply star.closure
+  intros x y h2
+  apply h1 at h2
+  apply star.singleton h2
+
+lemma conv.singleton {x y} : e x y -> conv e x y := by
+  intro h; apply conv.SE conv.R h
+
+lemma conv.singletoni {x y} : e y x -> conv e x y := by
+  intro h; apply conv.SEi conv.R h
+
+lemma conv.trans {y x z} : conv e x y -> conv e y z -> conv e x z := by
+  intros h1 h2
+  induction h2 with
+  | R => exact h1
+  | SE _ rel ih => apply conv.SE ih rel
+  | SEi _ rel ih => apply conv.SEi ih rel
+
+lemma conv.ES {x y z} : e x y -> conv e y z -> conv e x z := by
+  intro h
+  apply conv.trans
+  apply conv.singleton
+  assumption
+
+lemma conv.ESi {x y z} : e y x -> conv e y z -> conv e x z := by
+  intro h
+  apply conv.trans
+  apply conv.singletoni
+  assumption
+
+lemma conv.sym {x y} : conv e x y -> conv e y x := by
+  intro h
+  induction h with
+  | R => constructor
+  | SE _ rel ih => apply conv.ESi rel ih
+  | SEi _ rel ih => apply conv.ES rel ih
+
+lemma conv.join {x y z} : star e x y -> star e z y -> conv e x z := by
+  intro h1 h2
+  apply conv.trans
+  apply star.conv h1
+  apply conv.sym
+  apply star.conv h2
+
+lemma conv.img {T1 T2} {f : T1 -> T2} {e1 e2} :
+  (∀ {x y}, e1 x y -> conv e2 (f x) (f y)) ->
+  (∀ {x y}, conv e1 x y -> conv e2 (f x) (f y)) := by
+  intros h1 x y h2
+  induction h2 with
+  | R => aesop
+  | SE _ rel ih =>
+    apply conv.trans ih (h1 rel)
+  | SEi _ rel ih =>
+    apply conv.trans ih
+    apply conv.sym
+    apply h1 rel
+
+lemma conv.hom {T1 T2} (f : T1 -> T2) {e1 e2} :
+  (∀ {x y}, e1 x y -> e2 (f x) (f y)) ->
+  (∀ {x y}, conv e1 x y -> conv e2 (f x) (f y)) := by
+  intro h; apply conv.img
+  intros x y h0
+  apply h at h0
+  apply conv.singleton h0
+
+lemma confluent_cr : confluent e <-> CR e := by
+  constructor
+  . intro h1 x y h2
+    induction h2 with
+    | R => exists x; constructor <;> aesop
+    | @SE y z _ rel ih =>
+      rcases ih with ⟨u, ⟨h2, h3⟩⟩
+      rcases h1 h3 (star.singleton rel) with ⟨v, ⟨h4, h5⟩⟩
+      exists v; constructor
+      . apply star.trans h2 h4
+      . apply h5
+    | @SEi y z _ rel ih =>
+      rcases ih with ⟨u, ⟨h2, h3⟩⟩
+      exists u; constructor
+      . apply h2
+      . apply star.ES rel h3
+  . intro h x y z  h1 h2
+    apply star.conv at h1
+    apply star.conv at h2
+    apply h
+    apply conv.trans (conv.sym h1) h2
+
+lemma com.strip {e1 e2 : Rel T} : com e1 e2 -> com (star e2) e1 := by
+  intros h1 x y z h2
+  induction h2 with
+  | R => intro h2; exists z; aesop
+  | SE _ rel2 ih =>
+    intro h2
+    rcases ih h2 with ⟨u, ⟨rel1, h3⟩⟩
+    rcases h1 rel1 rel2 with ⟨v, ⟨rel2, rel1⟩⟩
+    exists v; constructor
+    . assumption
+    . apply star.SE h3 rel2
+
+lemma com.lift {e1 e2 : Rel T} : com e1 e2 -> com (star e1) (star e2) := by
+  intro h
+  apply com.strip at h
+  apply com.strip at h
+  assumption
+
+lemma diamond_confluent : diamond e -> confluent e := by
+  apply com.lift
+end ars_lemmas
